erasure/theories/ESubstitution.v
@@ -112,9 +112,9 @@ Proof.
     intros ? ? [[] [? []]].
     split; eauto.
   - econstructor.
-    induction H2; constructor.
-    induction X3; constructor; depelim X2; eauto.
-    depelim X1.
+    induction H3; constructor.
+    induction X2; constructor; depelim X1; eauto.
+    depelim X0.
     eapply All2_All_mix_left in a0; eauto.
     eapply All2_impl. exact a0.
     cbn. intros ? ? [? ?]. eauto.
@@ -316,10 +316,10 @@ Proof.
     rewrite (All2_length X3) in IH |- *.
     apply IH. apply IH'.
 
-  - econstructor. depelim H3.
-    depelim X4; repeat constructor.
-    depelim X2; cbn. now eapply hdef.
-    depelim X2. cbn. eapply All2_map.
+  - econstructor. depelim H4.
+    depelim X3; repeat constructor.
+    depelim X1; cbn. now eapply hdef.
+    depelim X1. cbn. eapply All2_map.
     ELiftSubst.solve_all.
 Qed.
 
@@ -585,9 +585,9 @@ Proof.
         eapply typing_wf_local.  eassumption.
     + econstructor.
       eapply is_type_subst; eauto.
-  - cbn. depelim H1.
+  - cbn. depelim H2.
     * cbn; constructor.
-      depelim H1. depelim X5; depelim X2; repeat constructor; cbn; eauto.
+      depelim H2. depelim X4; depelim X1; repeat constructor; cbn; eauto.
       ELiftSubst.solve_all.
     * constructor. eapply is_type_subst in X3; tea.
       now cbn in X3.
