erasure/theories/ErasureProperties.v
@@ -252,7 +252,7 @@ Proof.
     + subst types. eapply conv_context_app_same; auto.
     + subst types. eapply conv_context_wf_local_app; eauto.
     + assumption.
-  - econstructor. depelim H2; constructor. depelim X5; depelim X2; constructor; eauto.
+  - econstructor. depelim H3; constructor. depelim X4; depelim X1; constructor; eauto.
     solve_all.
 Qed.
 
@@ -411,8 +411,8 @@ Proof.
   f_equal.
   eapply fix_context_subst_instance. all: eauto.
 
-  - cbn; constructor. depelim H4.
-    depelim X2; depelim X5; repeat constructor; cbn; eauto.
+  - cbn; constructor. depelim H5.
+    depelim X1; depelim X4; repeat constructor; cbn; eauto.
     solve_all.
 Qed.
 
@@ -566,7 +566,7 @@ Section wellscoped.
     - now eapply nth_error_Some_length, Nat.ltb_lt in H0.
     - solve_all. destruct a as [s []], b.
       unfold test_def. len in i0. now rewrite i i0.
-    - depelim X1; solve_all; constructor; eauto.
+    - depelim X0; solve_all; constructor; eauto.
   Qed.
 
   Lemma welltyped_wellformed {Σ : global_env_ext} {wfΣ : wf Σ} {Γ a} : welltyped Σ Γ a -> wellformed Σ a.
