template-pcuic/theories/PCUICToTemplateCorrectness.v
@@ -2374,11 +2374,11 @@ Proof.
   - cbn. destruct p as [? []]; simp prim_type; cbn; econstructor; eauto.
     1,3,5: eapply trans_declared_constant; tea.
     all:cbn in *.
-    all:move: X0; rewrite /Ast.Env.primitive_invariants /primitive_invariants.
-    1-2:intros [s []]; exists s; split => //;
+    all:move: H1; rewrite /Ast.Env.primitive_invariants /primitive_invariants.
+    1-2:intros []; split => //;
     destruct cdecl as [ty [?|] ?]; cbn in *; subst; auto => //.
     intros []; split => //. rewrite H1 //. rewrite H2 //.
-    all:depelim X2; eauto. intros _. solve_all.
+    all:depelim X1; eauto. intros _. solve_all.
   - eapply TT.type_Conv.
     + eassumption.
     + eassumption.
